type/typecheck.v
@@ -15,23 +15,56 @@ Fixpoint lookup (c: (list (nat*local))) (m: nat): option local :=
 Print process.
 
 Inductive propcont: local -> Prop :=
-  | pc_inact: propcont ltinact
-  | pc_send : forall p l s c, propcont c -> propcont (ltsend p l s c)
-  | pc_recv : forall p C, List.Forall (fun u => propcont u) (map snd C) -> 
-                          propcont (ltreceive p C).
+  | prc_inact: propcont ltinact
+  | prc_send : forall p l s c, propcont c -> propcont (ltsend p l s c)
+  | prc_recv : forall p C, List.Forall (fun u => propcont u) (map snd C) -> 
+                           propcont (ltreceive p C).
+
+Inductive typecont: local -> Prop :=
+  | tyc_end   : typecont ltend
+  | tyc_send  : forall p l s c, typecont c -> typecont (ltselect p l s c)
+  | tyc_branch: forall p C, List.Forall (fun u => typecont u) (map snd C) -> 
+                            typecont (ltbranch p C).
 
 (* incomplete set of rules *)
 Inductive typeCheck: list (fin*local) -> fin -> local -> local -> Prop :=
   | tc_inact : forall m c, typeCheck c m (ltinact) (ltend)
-  | tc_var  : forall m c s t, Some t = lookup c s ->
+  | tc_end   : forall m c, typeCheck c m ltend ltstar
+  | tc_var   : forall m c s t, Some t = lookup c s ->
                               typeCheck c m (ltvar s) t
   | tc_lambda: forall c p k e t' n m, typeCheck c m p ltstar ->
                                       let t := betan n k (mkproc p gnil) in
                                       (* ctx ext *)
                                       typeCheck ((m, (@body t)) :: c) (S m) e t' ->
                                       typeCheck c m (ltlambda p e) (ltpi (@body t) t')
+  | tc_pair  : forall c p k e t' n m, typeCheck c m p ltstar ->
+                                      let t := betan n k (mkproc p gnil) in
+                                      (* ctx ext *)
+                                      typeCheck ((m, (@body t)) :: c) (S m) e t' ->
+                                      typeCheck c m (ltpair p e) (ltsig (@body t) t') 
   | tc_mu    : forall m c p t, typeCheck ((m, t) :: c) (S m) p t ->
                                typeCheck c m (ltmu t p) t
+  | tc_nval  : forall c m n, typeCheck c m (ltnval n) ltnat
+  | tc_bval  : forall c m b, typeCheck c m (ltbval b) ltbool
+  | tc_star  : forall c m, typeCheck c m ltstar ltstar
+  | tc_nat   : forall c m, typeCheck c m ltnat ltstar
+  | tc_bool  : forall c m, typeCheck c m ltbool ltstar
+  | tc_add   : forall c e1 e2 m, typeCheck c m e1 ltnat ->
+                                 typeCheck c m e2 ltnat ->
+                                 typeCheck c m (ltadd e1 e2) ltnat
+  | tc_mult  : forall c e1 e2 m, typeCheck c m e1 ltnat ->
+                                 typeCheck c m e2 ltnat ->
+                                 typeCheck c m (ltmult e1 e2) ltnat
+  | tc_subtr : forall c e1 e2 m, typeCheck c m e1 ltnat ->
+                                 typeCheck c m e2 ltnat ->
+                                 typeCheck c m (ltsubtr e1 e2) ltnat
+  | tc_ite   : forall c e1 e2 e3 t m, typeCheck c m e1 ltbool ->
+                                      typeCheck c m e2 t ->
+                                      typeCheck c m e3 t ->
+                                      typeCheck c m (ltite e1 e2 e3) t
+  | tc_gt    : forall c e1 e2 m, typeCheck c m e1 ltnat ->
+                                 typeCheck c m e2 ltnat ->
+                                 typeCheck c m (ltgt e1 e2) ltbool
   | tc_app   : forall c k e e' t t' n m, typeCheck c m e (ltpi t t') ->
                                          typeCheck c m e' t ->
                                          let tt := subst_local (e' .: ltvar) t' in
@@ -42,6 +75,11 @@ Inductive typeCheck: list (fin*local) -> fin -> local -> local -> Prop :=
                                                (* ctx ext *)
                                                typeCheck ((m, (@body t)) :: c) (S m) p' ltstar ->
                                                typeCheck c m (ltpi p p') ltstar
+  | tc_sig   : forall c k p p' (t: local) n m, typeCheck c m p ltstar ->
+                                               let t := betan n k (mkproc p gnil) in
+                                               (* ctx ext *)
+                                               typeCheck ((m, (@body t)) :: c) (S m) p' ltstar ->
+                                               typeCheck c m (ltsig p p') ltstar
   | tc_send  : forall m c p l e P S T, propcont P ->
                                        typeCheck c m e S ->
                                        typeCheck c m P T ->
@@ -53,4 +91,22 @@ Inductive typeCheck: list (fin*local) -> fin -> local -> local -> Prop :=
                       length P = length T ->
                       (* ctx ext *)
                       List.Forall (fun u => typeCheck ((m, (fst u)) :: c) (S m) (fst (snd u)) (snd (snd u))) (zip ST (zip P T)) ->
-                      typeCheck c m (ltreceive p (zip (zip L ST) P)) (ltbranch p (zip (zip L ST) T)).
+                      typeCheck c m (ltreceive p (zip (zip L ST) P)) (ltbranch p (zip (zip L ST) T))
+  | tc_branch: forall m c k p L (ST T: list local) n,
+                      List.Forall (fun u => typecont u) T -> 
+                      length L  = length ST ->
+                      length ST = length T ->
+                      List.Forall (fun u => typeCheck c m u ltstar) ST ->
+                      let ST' := betanList n k (mkprocL ST) in
+                      let ST'' := map (@body) ST' in
+                      (* ctx ext *)
+                      List.Forall (fun u => typeCheck ((m, (fst u)) :: c) (S m) (snd u) ltstar) (zip ST'' T) ->
+                      typeCheck c m (ltbranch p (zip (zip L ST) T)) ltstar
+  | tc_select: forall m c k p l ST T n,
+                      typecont T ->
+                      let ST' := betan n k (mkproc ST gnil) in
+                      (* ctx ext *)
+                      typeCheck ((m, (@body ST')) :: c) (S m) T ltstar ->
+                      typeCheck c m (ltselect p l ST T) ltstar.
+
+
