README.md
@@ -1,2 +1,0 @@
-# dependentDST
-An experimental development of session types + dependent types
